WeldAndArrow.lean
@@ -3,3 +3,4 @@
 import WeldAndArrow.Theory
 import WeldAndArrow.Theorems
 import WeldAndArrow.Identification
+import WeldAndArrow.Invariance
